stdlib/iterator/theories/iterator.v
@@ -1,2 +1,69 @@
 From refinedrust Require Import typing.
 
+Definition traits_iterator_Iterator_Inv_sig `{RRGS : !(refinedrustGS Σ)} (Self_rt: RT) (Item_rt: RT) :=
+  (thread_id → (RT_xt (Self_rt)) → iProp Σ).
+Definition traits_iterator_Iterator_Next_sig `{RRGS : !(refinedrustGS Σ)} (Self_rt: RT) (Item_rt: RT) (traits_iterator_Iterator_Inv: (traits_iterator_Iterator_Inv_sig (Self_rt) (Item_rt))) :=
+  (thread_id → (RT_xt (Self_rt)) → option (RT_xt (Item_rt)) → (RT_xt (Self_rt)) → iProp Σ).
+Record traits_iterator_Iterator_spec_attrs `{RRGS : !(refinedrustGS Σ)} `{Self_rt : !RT} `{Item_rt : !RT} : Type := mk_traits_iterator_Iterator_spec_attrs {
+  traits_iterator_Iterator_Inv  : (traits_iterator_Iterator_Inv_sig (Self_rt) (Item_rt));
+  traits_iterator_Iterator_Next  : (traits_iterator_Iterator_Next_sig (Self_rt) (Item_rt) (traits_iterator_Iterator_Inv));
+}.
+#[global] Arguments traits_iterator_Iterator_spec_attrs : clear implicits.
+#[global] Arguments traits_iterator_Iterator_spec_attrs {_ _}.
+#[global] Arguments mk_traits_iterator_Iterator_spec_attrs  {_} {_} {_} {_}.
+
+Section trans.
+  Context `{RRGS : !refinedrustGS Σ}.
+  (* Note: Depends on the whole attrs instead of the Next projection so that the projection doesn't simplify away, which is a problem for [LearnFromHyp] rules. *)
+  Fixpoint IteratorNextFusedTrans {Self_rt Item_rt : RT}
+    (attrs : traits_iterator_Iterator_spec_attrs Self_rt Item_rt)
+    (π : thread_id)
+    (s1 : RT_xt Self_rt) (els : list (RT_xt Item_rt)) (s2 : RT_xt Self_rt) : iProp Σ
+    :=
+    match els with
+    | [] => ⌜s1 = s2⌝
+    | (e1 :: els) =>
+      ∃ s1',
+        attrs.(traits_iterator_Iterator_Next) π s1 (Some e1) s1' ∗
+        IteratorNextFusedTrans attrs π s1' els s2
+    end.
+
+  Lemma iterator_next_fused_trans_app {Self_rt Item_rt : RT} (A : traits_iterator_Iterator_spec_attrs Self_rt Item_rt) π s1 hist s2 x :
+    IteratorNextFusedTrans A π s1 (hist ++ [x]) s2 ⊣⊢ (∃ s2', IteratorNextFusedTrans A π s1 hist s2' ∗ A.(traits_iterator_Iterator_Next) π s2' (Some x) s2).
+  Proof.
+    iInduction hist as [ | y hist] "IH" forall (s1 s2); simpl.
+    - iSplit.
+      + iIntros "(%s1' & ? & <-)". by iFrame.
+      + iIntros "(%s2' & -> & ?)". by iFrame.
+    - iSplit.
+      + iIntros "(%s1' & Ha & Hb)".
+        iPoseProof ("IH" with "Hb") as "(%s2' & Hb & Hc)".
+        iFrame.
+      + iIntros "(%s2' & (%s1' & ? & ?) & ?)".
+        iFrame. iApply "IH". iFrame.
+  Qed.
+
+  Lemma simplify_goal_iterator_next_fused_trans_app {Self_rt Item_rt : RT} (A : traits_iterator_Iterator_spec_attrs Self_rt Item_rt) π s1 hist s2 s1' hist' `{!CheckOwnInContext (IteratorNextFusedTrans A π s1 hist' s1')} T :
+    (∃ x,
+      ⌜hist = hist' ++ [x]⌝ ∗
+      IteratorNextFusedTrans A π s1 hist' s1' ∗
+      A.(traits_iterator_Iterator_Next) π s1' (Some x) s2) ∗ T ⊢ simplify_goal (IteratorNextFusedTrans A π s1 hist s2) T.
+  Proof.
+    rewrite /simplify_goal.
+    iIntros "((%x & -> & Ha & Hb) & $)".
+    rewrite iterator_next_fused_trans_app.
+    iFrame.
+  Qed.
+  Definition simplify_goal_iterator_next_fused_trans_app_inst := [instance @simplify_goal_iterator_next_fused_trans_app with 50%N].
+  Global Existing Instance simplify_goal_iterator_next_fused_trans_app_inst.
+
+  Lemma simplify_goal_iterator_next_fused_trans_nil {Self_rt Item_rt : RT} (A : traits_iterator_Iterator_spec_attrs Self_rt Item_rt) π s1 hist T :
+    (⌜hist = []⌝) ∗ T ⊢ simplify_goal (IteratorNextFusedTrans A π s1 hist s1) T.
+  Proof.
+    rewrite /simplify_goal.
+    iIntros "(-> & $)".
+    eauto.
+  Qed.
+  Definition simplify_goal_iterator_next_fused_trans_nil_inst := [instance @simplify_goal_iterator_next_fused_trans_nil with 10%N].
+  Global Existing Instance simplify_goal_iterator_next_fused_trans_nil_inst.
+End trans.
