stdlib/iterator/theories/map.v
@@ -1,4 +1,4 @@
-From refinedrust Require Import typing.
+From refinedrust Require Import typing shims.
 From rrstd.iterator.theories Require Import iterator.
 
 Record MapX (I : RT) (F : RT) : Type := mk_map_x {
@@ -46,3 +46,34 @@ Lemma li_sealed_use_pers `{!refinedrustGS Σ} (P : iProp Σ) `{!Persistent P} :
 Proof.
   unfold li_sealed. iIntros "#Ha". iModIntro. done.
 Qed.
+
+Section map.
+  Context `{RRGS : !refinedrustGS Σ}.
+  Definition MapInv {Self_rt Item_rt Clos_rt Clos_out_rt : RT} 
+    (iter_attrs : traits_iterator_Iterator_spec_attrs Self_rt Item_rt)
+    (Pre : thread_id → RT_xt Clos_rt → RT_xt (tuple1_rt Item_rt) → iProp Σ)
+    (PostMut : thread_id → RT_xt Clos_rt → RT_xt (tuple1_rt Item_rt) → RT_xt Clos_rt → RT_xt Clos_out_rt → iProp Σ) 
+    (*(fnonce_attrs : FnOnce_spec_attrs Clos_rt (tuple1_rt Item_rt) Clos_out_rt)*)
+    (*(fnmut_attrs : FnMut_spec_attrs Clos_rt (tuple1_rt Item_rt) Clos_out_rt) *)
+    : _ → _ → iProp Σ := 
+    λ (π : thread_id) (s : MapX Self_rt Clos_rt),
+    (∃ (Inv : thread_id → RT_xt Self_rt → RT_xt Clos_rt → iProp Σ),
+      (* user-picked invariant *)
+      Inv π s.(map_it) s.(map_clos) ∗
+      (* nested iterator invariant *)
+      iter_attrs.(traits_iterator_Iterator_Inv) π s.(map_it) ∗
+      (* progress *)
+      li_sealed (□ (∀ it_state it_state' clos_state e,
+        iter_attrs.(traits_iterator_Iterator_Next) π it_state (Some e) it_state' -∗
+        Inv π it_state clos_state -∗
+        Pre π clos_state *[e] ∗
+        (∀ e' clos_state', PostMut π clos_state *[e] clos_state' e' -∗ Inv π it_state' clos_state'))) ∗
+      (* progress (no element) *)
+      li_sealed (□ (∀ it_state it_state' clos_state,
+        iter_attrs.(traits_iterator_Iterator_Next) π it_state None it_state' -∗
+        Inv π it_state clos_state -∗
+        Inv π it_state' clos_state)))%I.
+
+  Global Arguments MapInv : simpl never.
+  Global Typeclasses Opaque MapInv.
+End map.
