stdlib/iterator/output/iterator/proofs/proof_adapters_map_MapMIMFastraits_iterator_Iterator_next.v
@@ -1,16 +1,16 @@
 From caesium Require Import lang notation.
 From refinedrust Require Import typing shims.
-From rrstd.iterator.iterator.generated Require Import generated_code_iterator generated_specs_iterator generated_template_adapters_map_MapMBMIMFastraits_iterator_Iterator_next.
+From rrstd.iterator.iterator.generated Require Import generated_code_iterator generated_specs_iterator generated_template_adapters_map_MapMIMFastraits_iterator_Iterator_next.
 
 Set Default Proof Using "Type".
 
 Section proof.
 Context `{RRGS : !refinedrustGS Σ}.
 
-Lemma adapters_map_MapMBMIMFastraits_iterator_Iterator_next_proof (π : thread_id) :
-  adapters_map_MapMBMIMFastraits_iterator_Iterator_next_lemma π.
+Lemma adapters_map_MapMIMFastraits_iterator_Iterator_next_proof (π : thread_id) :
+  adapters_map_MapMIMFastraits_iterator_Iterator_next_lemma π.
 Proof.
-  adapters_map_MapMBMIMFastraits_iterator_Iterator_next_prelude.
+  adapters_map_MapMIMFastraits_iterator_Iterator_next_prelude.
 
   rep liRStep. liShow.
 
@@ -31,20 +31,21 @@ Proof.
     iRename select (FnMut_PostMut _ _ _ _ _ _) into "Hpost".
     iPoseProof (boringly_intro with "Hpost") as "#Hpost_x".
     iPoseProof ("Hinv_clos" with "Hpost") as "Hinv".
-    rep liRStep.
-    liInst Hevar (mut_ref_ghost_drop _ _).
-    liInst Hevar2 x4.
     rep liRStep. liShow.
+    liInst Hevar (mut_ref_ghost_drop _ _).
     iApply prove_with_subtype_default.
-    liInst Hevar r.
-    rep liRStep. }
+    liInst Hevar0 r.
+    rep liRStep. 
+    liInst Hevar x4.
+    rep liRStep.
+  }
   { (* no element *)
     iPoseProof ("Hnone'" with "Hnext Hinv") as "Hinv".
     simpl.
     rep <-! liRStep. liShow. 
     rep 100 liRStep. liShow.
     rep liRStep.
-    liInst Hevar1 x4.
+    liInst Hevar x4.
     rep liRStep. }
 
   all: print_remaining_goal.
