stdlib/iterator/output/iterator/proofs/proof_adapters_map_Map_IF_new.v
@@ -1,19 +1,17 @@
 From caesium Require Import lang notation.
 From refinedrust Require Import typing shims.
-From rrstd.iterator.iterator.generated Require Import generated_code_iterator generated_specs_iterator generated_template_adapters_map_Map_BIF_new.
+From rrstd.iterator.iterator.generated Require Import generated_code_iterator generated_specs_iterator generated_template_adapters_map_Map_IF_new.
 
 Set Default Proof Using "Type".
 
 Section proof.
 Context `{RRGS : !refinedrustGS Σ}.
 
-Lemma adapters_map_Map_BIF_new_proof (π : thread_id) :
-  adapters_map_Map_BIF_new_lemma π.
+Lemma adapters_map_Map_IF_new_proof (π : thread_id) :
+  adapters_map_Map_IF_new_lemma π.
 Proof.
-  adapters_map_Map_BIF_new_prelude.
+  adapters_map_Map_IF_new_prelude.
 
-  repeat liRStep; liShow.
-  liInst Hevar Inv.
   repeat liRStep; liShow.
 
   all: print_remaining_goal.
