stdlib/iterator/output/iterator/proofs/proof_traits_iterator_Iterator_map.v
@@ -1,0 +1,33 @@
+From caesium Require Import lang notation.
+From refinedrust Require Import typing shims.
+From rrstd.iterator.iterator.generated Require Import generated_code_iterator generated_specs_iterator generated_template_traits_iterator_Iterator_map.
+
+Set Default Proof Using "Type".
+
+Section proof.
+Context `{RRGS : !refinedrustGS Σ}.
+
+Lemma traits_iterator_Iterator_map_proof (π : thread_id) :
+  traits_iterator_Iterator_map_lemma π.
+Proof.
+  traits_iterator_Iterator_map_prelude.
+
+  repeat liRStep; liShow.
+  unfold MapInv.
+  repeat liRStep; liShow.
+  liInst Hevar Inv.
+  iApply prove_with_subtype_default.
+  iFrame.
+  rep liRStep. liShow.
+  iApply prove_with_subtype_default.
+  iSplitR. { unfold li_sealed. done. }
+  iApply prove_with_subtype_default.
+  iSplitR. { unfold li_sealed. done. }
+  rep liRStep.
+
+  all: print_remaining_goal.
+  Unshelve. all: sidecond_solver.
+  Unshelve. all: sidecond_hammer.
+  Unshelve. all: print_remaining_sidecond.
+Qed.
+End proof.
